
\begin{question}
Основная гипотеза модели адаптивных ожиданий состоит в том, что
\begin{answerlist}[2]
  \item \(X_t^e - X_{t-1}^e = (1-\lambda) (X_t - X_{t-1}), \; 0 \leq \lambda < 1\)
  \item \(Y_t^e = \left(1 - \frac{1}{\delta}\right) Y_{t-1} + \frac{1}{\delta} Y_{t}, \; 0 < \delta \leq 1\)
  \item \(Y_t - Y_{t-1}^e = \delta (Y_t^e - Y_{t-1}), \; 0 < \delta \leq 1\)
  \item \(X_{t+1}^e - X_{t}^e = \lambda (X_{t} - X_{t}^e), \; 0 \leq \lambda < 1\)
  \item \(Y_t - Y_{t-1} = \delta (Y_t^e - Y_{t-1}), \; 0 < \delta \leq 1\)
\end{answerlist}
\end{question}


